array

theories/WPArray.v
@@ -1,6 +1,6 @@
 (**
 
-Formalization of arrays.
+Formalization of arrays, with lifting.
 
 Author: Arthur Charguéraud.
 License: CC-by 4.0.
@@ -9,17 +9,13 @@ License: CC-by 4.0.
 
 Set Implicit Arguments.
 From TLC Require LibListZ.
-From Sep Require Import LambdaCF LibSepTLCbuffer.
-Export NotationForVariables NotationForTerms.
+From Sep Require Export WPArrayNonLifted.
+Generalizable Variables A B.
+
+Import NotationForVariables NotationForTerms.
+Open Scope val_scope.
+Open Scope pat_scope.
 Open Scope trm_scope.
-Open Scope heap_scope.
-Open Scope liblist_scope.
-Open Scope charac.
-
-Ltac auto_star ::= jauto.
-
-
-Local Open Scope fmap_scope.
 
 Implicit Types t : trm.
 Implicit Types v : val.
@@ -29,219 +25,8 @@ Implicit Type l p q : loc.
 Implicit Types n : int.
 
 
-
-(* ********************************************************************** *)
-(* * Formalisation of arrays *)
-
-(* ---------------------------------------------------------------------- *)
-(** Representation *)
-
-Fixpoint Array (L:list val) (p:loc) : hprop :=
-  match L with
-  | nil => \[]
-  | x::L' => (p ~~~> x) \* (Array L' (S p))
-  end.
-
-Lemma Array_nil_eq : forall p,
-  Array nil p = \[].
-Proof using. auto. Qed.
-
-Lemma Array_cons_eq : forall p x L,
-  Array (x::L) p = (p ~~~> x) \* Array L (S p).
-Proof using. auto. Qed.
-
-Lemma Array_one_eq : forall p x,
-  Array (x::nil) p = (p ~~~> x).
-Proof using. intros. rewrite Array_cons_eq, Array_nil_eq. rew_heap~. Qed.
-
-Lemma Array_concat_eq : forall p L1 L2,
-  Array (L1++L2) p = Array L1 p \* Array L2 (p + length L1)%nat.
-Proof using.
-  Transparent loc.
-  intros. gen p. induction L1; intros; rew_list.
-  { rewrite Array_nil_eq. rew_heap. fequals. unfold loc; math. }
-  { do 2 rewrite Array_cons_eq. rewrite IHL1. rew_heap. do 3 fequals.
-    unfold loc; math. }
-Qed.
-
-Lemma Array_last_eq : forall p x L,
-  Array (L&x) p = Array L p \* ((p + length L)%nat ~~~> x).
-Proof using. intros. rewrite Array_concat_eq. rewrite~ Array_one_eq. Qed.
-
-Lemma Array_middle_eq : forall n p L,
-  0 <= n < length L ->
-  Array L p = \exists L1 x L2, \[L = L1++x::L2] \* \[length L1 = n :> int] \*
-    Array L1 p \* (abs(p+n) ~~~> x) \* Array L2 (p + length L1 + 1)%nat.
-Proof using.
-  (* LATER: simplify the Z/nat math, by using a result from LibListZ directly *)
-  introv N. applys himpl_antisym.
-  { forwards (L1&x&L2&E&HM): list_middle_inv (abs n) L.
-    asserts (N1&N2): (0 <= abs n /\ (abs n < length L)%Z).
-    { split; rewrite abs_nonneg; math. } math.
-    lets M': eq_int_of_eq_nat HM. rewrite abs_nonneg in M'; [|math].
-    xsimpl~ (>> L1 x L2). subst L. rewrite Array_concat_eq, Array_cons_eq.
-    rew_nat. xsimpl. rewrite HM. rewrite~ abs_nat_plus_nonneg. math. }
-  { xpull ;=> L1 x L2 HM E. subst n.
-    subst L. rewrite Array_concat_eq, Array_cons_eq.
-    rew_nat. xsimpl. applys_eq himpl_refl. fequals.
-    rewrite abs_nat_plus_nonneg; [|math]. rewrite~ abs_nat. }
-Qed.
-
-Global Opaque Array.
-
-
-(* ---------------------------------------------------------------------- *)
-(** Array allocation *)
-
-Lemma Array_of_Alloc : forall k l,
-  Alloc k l ==>
-  \exists (L : list val), \[length L = k] \* Array L l.
-Proof using.
-  intros. gen l. induction k; intros.
-  { rew_Alloc. xsimpl (@nil val). rew_list~. }
-  { rew_Alloc. xpull ;=> v. xchange IHk. xpull ;=> L E.
-    xsimpl (v::L).
-    { rewrite Array_cons_eq. xsimpl~. }
-    { rew_list. math. } }
-Qed.
-
-Lemma triple_alloc_array : forall n,
-  n >= 0 ->
-  triple (val_alloc n)
-    \[]
-    (fun r => \exists (p:loc) (L:list val), \[r = val_loc p] \*
-              \[length L = n :> int] \* Array L p).
-Proof using.
-  introv N. xapp. math.
-  intros r. xpull ;=> l (E&Nl). subst r.
-  xchange Array_of_Alloc. xpull ;=> L HL.
-  xsimpl~. rewrite HL. rewrite~ abs_nonneg.
-Qed.
-
-
-(* -------------------------------------------------------------------------- *)
-(** Accesses *)
-
-Import LibListZ.
-Implicit Types i ofs len : int.
-
-
-(* ---------------------------------------------------------------------- *)
-(** Array get *)
-
-Definition val_array_get : val :=
-  ValFun 'p 'i :=
-    Let 'n := val_ptr_add 'p 'i in
-    val_get 'n.
-
-Lemma triple_array_get : forall p i L,
-  index L i ->
-  triple (val_array_get p i)
-    (Array L p)
-    (fun r => \[r = L[i]] \* Array L p).
-Proof using.
-  introv N. rewrite index_eq_inbound in N.
-  xcf. xapps. { math. }
-  rewrites (>> Array_middle_eq i). { math. }
-  xtpull ;=> L1 x L2 EL HL.
-  xapp. xpull ;=> r. intro_subst.
-  xsimpl; auto. { subst. rewrite~ read_middle. }
-Qed.
-
-Hint Extern 1 (Register_spec val_array_get) => Provide triple_array_get.
-
-Notation "'Array'' p `[ i ]" := (trm_app (trm_app (trm_val val_array_get) p) i)
-  (at level 69, p at level 0, no associativity,
-   format "'Array''  p `[ i ]") : charac.
-
-
-(* ---------------------------------------------------------------------- *)
-(** Array set *)
-
-Definition val_array_set : val :=
-  ValFun 'p 'i 'x :=
-    Let 'n := val_ptr_add 'p 'i in
-    val_set 'n 'x.
-
-Lemma triple_array_set : forall p i v L,
-  index L i ->
-  triple (val_array_set p i v)
-    (Array L p)
-    (fun r => \[r = val_unit] \* Array (L[i:=v]) p).
-Proof using.
-  introv N. rewrite index_eq_inbound in N.
-  xcf. xapps. { math. }
-  rewrites (>> Array_middle_eq i). { math. }
-  xtpull ;=> L1 x L2 EL HL.
-  xapp triple_set. xpull ;=> r. intro_subst.
-  rewrites (>> Array_middle_eq i (L[i := v])).
-   { rewrite <- length_eq in *. rew_array. math. }
-  xsimpl; auto. { subst. rewrite~ update_middle. rew_list~. }
-Qed.
-
-Hint Extern 1 (Register_spec val_array_set) => Provide triple_array_set.
-
-Notation "'Array'' p `[ i ] `<- x" := (trm_app (trm_app (trm_app (trm_val val_array_set) p) i) x)
-  (at level 69, p at level 0, no associativity,
-   format "'Array''  p `[ i ]  `<-  x") : charac.
-
-
-(* ---------------------------------------------------------------------- *)
-(** Array make *)
-
-Definition val_array_make : val :=
-  ValFun 'n 'v :=
-    Let 'p := val_alloc 'n in
-    Let 'b := 'n '- 1 in
-    For 'i := 0 To 'b Do
-      Array' 'p`['i] `<- 'v
-    Done;;;
-    'p.
-
-Lemma triple_array_make : forall n v,
-  n >= 0 ->
-  triple (val_array_make n v)
-    \[]
-    (fun r => \exists p L, \[r = val_loc p] \* \[L = make n v] \* Array L p).
-Proof using.
-  introv N. xcf. xapp~ triple_alloc_array ;=> r p L Er EL. subst r.
-  xapps. xseq.
-  { (* LATER: xfor tactic *)
-    applys mklocal_erase. esplit; esplit; splits; [reflexivity|reflexivity|].
-    intros S LS EF M. subst EF. simpl in M.
-    cuts G: (forall i L', i >= 0 -> length L' = n-i ->
-       S i (Array ((make i v)++L') p) (fun r => (Array (make n v) p))).
-    { applys_eq (>> G L). math. math. rewrite make_zero. rew_list~. }
-    intros i. induction_wf IH: (upto n) i. intros L' Ei EL'.
-    applys (rm M). case_if.
-    { xseq. (* later: remove *)
-      xapp~. { rewrite index_eq_inbound. rew_list. rewrite length_make; math. }
-      intros r. xsimpl.
-      destruct L' as [|x L']. { false. rew_list in EL'. math. }
-      rewrite~ update_middle; [| rewrite length_make; math ].
-      rew_list. xapplys (>> IH L').
-      { auto with maths. }
-      { rew_list; math. }
-      { rew_list in *; math. }
-      { applys LS. }
-      { rewrite make_succ_r; [|math]. rew_list. xsimpl~. } }
-    { xval. math E: (i = LibList.length L).
-      asserts: (L' = nil). { applys length_zero_inv. math. }
-      subst. rew_list. xsimpl~. } }
-  { simpl ;=> _. xval. subst n. xsimpl~. }
-Qed.
-
-Hint Extern 1 (Register_spec val_array_make) => Provide triple_array_make.
-
-
-(* ---------------------------------------------------------------------- *)
-(** Array init *)
-
-
-
 (* ********************************************************************** *)
 (* * Lifted access rules for arrays *)
-
 
 (* ---------------------------------------------------------------------- *)
 (** Representation *)
@@ -265,8 +50,8 @@ Context A `{EA:Enc A}.
 Implicit Types L : list A.
 Implicit Types x : A.
 
-Lemma Array_eq_ArrayNonlifted : forall L p,
-  Array L p = LambdaStruct.Array (LibList.map enc L) p.
+Lemma Array_eq_array : forall L p,
+  Array L p = aArray (LibList.map enc L) p.
 Proof using.
   intros L. induction L; intros.
   { auto. }
@@ -274,8 +59,8 @@ Proof using.
 Qed.
 
 Lemma Array_unlift : forall L p,
-  p ~> Array L = LambdaStruct.Array (LibList.map enc L) p.
-Proof using. apply Array_eq_ArrayNonlifted. Qed.
+  p ~> Array L = array (LibList.map enc L) p.
+Proof using. apply Array_eq_array. Qed.
 
 Lemma Array_nil_eq : forall p,
   p ~> Array (@nil A)  = \[].
@@ -358,8 +143,6 @@ Proof using.
   unfold LiftPost. subst. xsimpl*.
 Qed.
 
-Hint Extern 1 (Register_Spec val_array_get) => Provide Triple_array_get.
-
 Lemma Triple_array_set : forall p i v L,
   index L i ->
   Triple (val_array_set ``p ``i ``v)
@@ -372,8 +155,6 @@ Proof using.
   unfold LiftPost. subst. rewrite Array_unlift. xsimpl~ tt.
 Qed.
 
-Hint Extern 1 (Register_Spec val_array_set) => Provide Triple_array_set.
-
 Lemma Triple_array_make : forall n v,
   n >= 0 ->
   Triple (val_array_make ``n ``v)
@@ -385,6 +166,8 @@ Proof using.
   rewrite Array_unlift. subst L. rewrite map_make; [|math]. xsimpl.
 Qed.
 
-Hint Extern 1 (Register_Spec val_array_make) => Provide Triple_array_make.
-
 End ArrayRules.
+
+Hint Extern 1 (Register_Spec val_array_get) => Provide Triple_array_get.
+Hint Extern 1 (Register_Spec val_array_set) => Provide Triple_array_set.
+Hint Extern 1 (Register_Spec val_array_make) => Provide Triple_array_make.
